{-# OPTIONS --without-K --exact-split #-}

module 05-identity-types where

import 04-inductive-types
open 04-inductive-types public

-- Section 5.1

-- Definition 5.1.1

{- We introduce the identity type. -}

data Id {i : Level} {A : UU i} (x : A) : A → UU i where
  refl : Id x x

{- In the following definition we give a construction of path induction.
   However, in the development of this library we will mostly use Agda's
   built-in methods to give constructions by path induction. -}

ind-Id :
  {i j : Level} {A : UU i} (x : A) (B : (y : A) (p : Id x y) → UU j) →
  (B x refl) → (y : A) (p : Id x y) → B y p
ind-Id x B b y refl = b

-- Section 5.2 The groupoid structure of types

-- Definition 5.2.1

_∙_ :
  {i : Level} {A : UU i} {x y z : A} → Id x y → Id y z → Id x z
refl ∙ q = q

concat :
  {i : Level} {A : UU i} {x y : A} → Id x y → (z : A) → Id y z → Id x z
concat p z q = p ∙ q

-- Definition 5.2.2

inv :
  {i : Level} {A : UU i} {x y : A} → Id x y → Id y x
inv refl = refl

-- Definition 5.2.3

assoc :
  {i : Level} {A : UU i} {x y z w : A} (p : Id x y) (q : Id y z)
  (r : Id z w) → Id ((p ∙ q) ∙ r) (p ∙ (q ∙ r))
assoc refl q r = refl

-- Definition 5.2.4

left-unit :
  {i : Level} {A : UU i} {x y : A} {p : Id x y} → Id (refl ∙ p) p
left-unit = refl

right-unit :
  {i : Level} {A : UU i} {x y : A} {p : Id x y} → Id (p ∙ refl) p
right-unit {p = refl} = refl

-- Definition 5.2.5

left-inv :
  {i : Level} {A : UU i} {x y : A} (p : Id x y) →
  Id ((inv p) ∙ p) refl
left-inv refl = refl

right-inv :
  {i : Level} {A : UU i} {x y : A} (p : Id x y) →
  Id (p ∙ (inv p)) refl
right-inv refl = refl

-- Section 5.3 The action on paths of functions

-- Definition 5.3.1

ap :
  {i j : Level} {A : UU i} {B : UU j} (f : A → B) {x y : A} (p : Id x y) →
  Id (f x) (f y)
ap f refl = refl

ap-id :
  {i : Level} {A : UU i} {x y : A} (p : Id x y) → Id (ap id p) p
ap-id refl = refl

ap-comp :
  {i j k : Level} {A : UU i} {B : UU j} {C : UU k} (g : B → C)
  (f : A → B) {x y : A} (p : Id x y) → Id (ap (g ∘ f) p) (ap g (ap f p))
ap-comp g f refl = refl

-- Definition 5.3.2

ap-refl :
  {i j : Level} {A : UU i} {B : UU j} (f : A → B) (x : A) →
  Id (ap f (refl {_} {_} {x})) refl
ap-refl f x = refl

ap-concat :
  {i j : Level} {A : UU i} {B : UU j} (f : A → B) {x y z : A}
  (p : Id x y) (q : Id y z) → Id (ap f (p ∙ q)) ((ap f p) ∙ (ap f q))
ap-concat f refl q = refl

ap-inv :
  {i j : Level} {A : UU i} {B : UU j} (f : A → B) {x y : A}
  (p : Id x y) → Id (ap f (inv p)) (inv (ap f p))
ap-inv f refl = refl

-- Section 5.4 Transport

-- Definition 5.4.1

tr :
  {i j : Level} {A : UU i} (B : A → UU j) {x y : A} (p : Id x y) → B x → B y
tr B refl b = b

-- Definition 5.4.2

apd :
  {i j : Level} {A : UU i} {B : A → UU j} (f : (x : A) → B x) {x y : A}
  (p : Id x y) → Id (tr B p (f x)) (f y)
apd f refl = refl

path-over :
  {i j : Level} {A :  UU i} (B : A → UU j) {x x' : A} (p : Id x x') →
  B x → B x' → UU j
path-over B p y y' = Id (tr B p y) y'

refl-path-over :
  {i j : Level} {A : UU i} (B : A → UU j) (x : A) (y : B x) →
  path-over B refl y y
refl-path-over B x y = refl

-- Exercises

-- Exercise 5.1

-- Exercise 5.2

distributive-inv-concat :
  {i : Level} {A : UU i} {x y : A} (p : Id x y) {z : A}
  (q : Id y z) → Id (inv (p ∙ q)) ((inv q) ∙ (inv p))
distributive-inv-concat refl refl = refl

-- Exercise 5.3

inv-con :
  {i : Level} {A : UU i} {x y : A} (p : Id x y) {z : A} (q : Id y z)
  (r : Id x z) → (Id (p ∙ q) r) → Id q ((inv p) ∙ r)
inv-con refl q r = id 

con-inv :
  {i : Level} {A : UU i} {x y : A} (p : Id x y) {z : A} (q : Id y z)
  (r : Id x z) → (Id (p ∙ q) r) → Id p (r ∙ (inv q))
con-inv p refl r =
  ( λ α → α ∙ (inv right-unit)) ∘ (concat (inv right-unit) r)

-- Exercise 5.4

lift :
  {i j : Level} {A : UU i} {B : A → UU j} {x y : A} (p : Id x y)
  (b : B x) → Id (pair x b) (pair y (tr B p b))
lift refl b = refl

-- Exercise 5.5

-- Exercise 5.5(a)

abstract
  right-unit-law-add-ℕ :
    (x : ℕ) → Id (add-ℕ x zero-ℕ) x
  right-unit-law-add-ℕ x = refl
  
  left-unit-law-add-ℕ :
    (x : ℕ) → Id (add-ℕ zero-ℕ x) x
  left-unit-law-add-ℕ zero-ℕ = refl
  left-unit-law-add-ℕ (succ-ℕ x) = ap succ-ℕ (left-unit-law-add-ℕ x)
  
  left-successor-law-add-ℕ :
    (x y : ℕ) → Id (add-ℕ (succ-ℕ x) y) (succ-ℕ (add-ℕ x y))
  left-successor-law-add-ℕ x zero-ℕ = refl
  left-successor-law-add-ℕ x (succ-ℕ y) =
    ap succ-ℕ (left-successor-law-add-ℕ x y)

  right-successor-law-add-ℕ :
    (x y : ℕ) → Id (add-ℕ x (succ-ℕ y)) (succ-ℕ (add-ℕ x y))
  right-successor-law-add-ℕ x y = refl

-- Exercise 5.5(b)

abstract
  associative-add-ℕ :
    (x y z : ℕ) → Id (add-ℕ (add-ℕ x y) z) (add-ℕ x (add-ℕ y z))
  associative-add-ℕ x y zero-ℕ = refl 
  associative-add-ℕ x y (succ-ℕ z) = ap succ-ℕ (associative-add-ℕ x y z)

abstract
  commutative-add-ℕ : (x y : ℕ) → Id (add-ℕ x y) (add-ℕ y x)
  commutative-add-ℕ zero-ℕ y = left-unit-law-add-ℕ y
  commutative-add-ℕ (succ-ℕ x) y =
    (left-successor-law-add-ℕ x y) ∙ (ap succ-ℕ (commutative-add-ℕ x y))

-- Exercise 5.5(c)

abstract
  left-zero-law-mul-ℕ :
    (x : ℕ) → Id (mul-ℕ zero-ℕ x) zero-ℕ
  left-zero-law-mul-ℕ x = refl

  right-zero-law-mul-ℕ :
    (x : ℕ) → Id (mul-ℕ x zero-ℕ) zero-ℕ
  right-zero-law-mul-ℕ zero-ℕ = refl
  right-zero-law-mul-ℕ (succ-ℕ x) =
    ( right-unit-law-add-ℕ (mul-ℕ x zero-ℕ)) ∙ (right-zero-law-mul-ℕ x)

abstract
  right-unit-law-mul-ℕ :
    (x : ℕ) → Id (mul-ℕ x one-ℕ) x
  right-unit-law-mul-ℕ zero-ℕ = refl
  right-unit-law-mul-ℕ (succ-ℕ x) = ap succ-ℕ (right-unit-law-mul-ℕ x)

  left-unit-law-mul-ℕ :
    (x : ℕ) → Id (mul-ℕ one-ℕ x) x
  left-unit-law-mul-ℕ zero-ℕ = refl
  left-unit-law-mul-ℕ (succ-ℕ x) = ap succ-ℕ (left-unit-law-mul-ℕ x)

abstract
  left-successor-law-mul-ℕ :
    (x y : ℕ) → Id (mul-ℕ (succ-ℕ x) y) (add-ℕ (mul-ℕ x y) y)
  left-successor-law-mul-ℕ x y = refl

  right-successor-law-mul-ℕ :
    (x y : ℕ) → Id (mul-ℕ x (succ-ℕ y)) (add-ℕ x (mul-ℕ x y))
  right-successor-law-mul-ℕ zero-ℕ y = refl
  right-successor-law-mul-ℕ (succ-ℕ x) y =
    ( ( ap (λ t → succ-ℕ (add-ℕ t y)) (right-successor-law-mul-ℕ x y)) ∙
      ( ap succ-ℕ (associative-add-ℕ x (mul-ℕ x y) y))) ∙
    ( inv (left-successor-law-add-ℕ x (add-ℕ (mul-ℕ x y) y)))

-- Exercise 5.5(d)

abstract
  commutative-mul-ℕ :
    (x y : ℕ) → Id (mul-ℕ x y) (mul-ℕ y x)
  commutative-mul-ℕ zero-ℕ y = inv (right-zero-law-mul-ℕ y)
  commutative-mul-ℕ (succ-ℕ x) y =
    ( commutative-add-ℕ (mul-ℕ x y) y) ∙ 
    ( ( ap (add-ℕ y) (commutative-mul-ℕ x y)) ∙
      ( inv (right-successor-law-mul-ℕ y x)))

-- Exercise 5.5(e)

abstract
  left-distributive-mul-add-ℕ :
    (x y z : ℕ) → Id (mul-ℕ x (add-ℕ y z)) (add-ℕ (mul-ℕ x y) (mul-ℕ x z))
  left-distributive-mul-add-ℕ zero-ℕ y z = refl
  left-distributive-mul-add-ℕ (succ-ℕ x) y z =
    ( left-successor-law-mul-ℕ x (add-ℕ y z)) ∙ 
    ( ( ap (λ t → add-ℕ t (add-ℕ y z)) (left-distributive-mul-add-ℕ x y z)) ∙ 
      ( ( associative-add-ℕ (mul-ℕ x y) (mul-ℕ x z) (add-ℕ y z)) ∙
        ( ( ap ( add-ℕ (mul-ℕ x y)) 
               ( ( inv (associative-add-ℕ (mul-ℕ x z) y z)) ∙
                 ( ( ap (λ t → add-ℕ t z) (commutative-add-ℕ (mul-ℕ x z) y)) ∙
                   ( associative-add-ℕ y (mul-ℕ x z) z)))) ∙ 
          ( inv (associative-add-ℕ (mul-ℕ x y) y (add-ℕ (mul-ℕ x z) z))))))

abstract
  right-distributive-mul-add-ℕ :
    (x y z : ℕ) → Id (mul-ℕ (add-ℕ x y) z) (add-ℕ (mul-ℕ x z) (mul-ℕ y z))
  right-distributive-mul-add-ℕ x y z =
    ( commutative-mul-ℕ (add-ℕ x y) z) ∙ 
    ( ( left-distributive-mul-add-ℕ z x y) ∙ 
      ( ( ap (λ t → add-ℕ t (mul-ℕ z y)) (commutative-mul-ℕ z x)) ∙ 
        ( ap (λ t → add-ℕ (mul-ℕ x z) t) (commutative-mul-ℕ z y))))

-- Exercise 5.5(f)

abstract
  associative-mul-ℕ :
    (x y z : ℕ) → Id (mul-ℕ (mul-ℕ x y) z) (mul-ℕ x (mul-ℕ y z))
  associative-mul-ℕ zero-ℕ y z = refl
  associative-mul-ℕ (succ-ℕ x) y z =
    ( right-distributive-mul-add-ℕ (mul-ℕ x y) y z) ∙ 
    ( ap (λ t → add-ℕ t (mul-ℕ y z)) (associative-mul-ℕ x y z))

-- Exercise 5.6

Mac-Lane-pentagon :
  {i : Level} {A : UU i} {a b c d e : A}
  (p : Id a b) (q : Id b c) (r : Id c d) (s : Id d e) →
  let α₁ = (ap (λ t → t ∙ s) (assoc p q r))
      α₂ = (assoc p (q ∙ r) s)
      α₃ = (ap (λ t → p ∙ t) (assoc q r s))
      α₄ = (assoc (p ∙ q) r s)
      α₅ = (assoc p q (r ∙ s))
  in
  Id ((α₁ ∙ α₂) ∙ α₃) (α₄ ∙ α₅)
Mac-Lane-pentagon refl refl refl refl = refl


{- The following code is an experiment that shows that constructions in an
   abstract environment do remember the specific definitions of previous
   definitions in abstract environments. -}

abstract
  abstract-concat :
    {l : Level} {A : UU l} {x y z : A} → Id x y → Id y z → Id x z
  abstract-concat refl q = q

  abstract-left-unit-law :
    {l : Level} {A : UU l} {x y : A} (q : Id x y) → Id (abstract-concat refl q) q
  abstract-left-unit-law q = refl

{- We just make some random definition to make sure that we are not in the 
   same abstract envirnoment anymore. -}
one : ℕ
one = succ-ℕ zero-ℕ

abstract
  abstract-right-unit-law :
    {l : Level} {A : UU l} {x y : A} (p : Id x y) →
      Id (abstract-concat p refl) p
  abstract-right-unit-law refl = refl

  {- The term refl should not be accepted if the definition of abstract-concat
     were forgotten. A definition that would work under all circumstances is
     abstract-left-unit refl. -}

-- The ring axioms for ℤ

abstract
  left-inverse-pred-ℤ :
    (k : ℤ) → Id (pred-ℤ (succ-ℤ k)) k
  left-inverse-pred-ℤ (inl zero-ℕ) = refl
  left-inverse-pred-ℤ (inl (succ-ℕ x)) = refl
  left-inverse-pred-ℤ (inr (inl star)) = refl
  left-inverse-pred-ℤ (inr (inr zero-ℕ)) = refl
  left-inverse-pred-ℤ (inr (inr (succ-ℕ x))) = refl

  right-inverse-pred-ℤ :
    (k : ℤ) → Id (succ-ℤ (pred-ℤ k)) k
  right-inverse-pred-ℤ (inl zero-ℕ) = refl
  right-inverse-pred-ℤ (inl (succ-ℕ x)) = refl
  right-inverse-pred-ℤ (inr (inl star)) = refl
  right-inverse-pred-ℤ (inr (inr zero-ℕ)) = refl
  right-inverse-pred-ℤ (inr (inr (succ-ℕ x))) = refl

{- Exercise 6.12 (a) simply asks to prove the unit laws. The left unit law
   holds by judgmental equality. -}

abstract
  left-unit-law-add-ℤ :
    (k : ℤ) → Id (add-ℤ zero-ℤ k) k
  left-unit-law-add-ℤ k = refl

  right-unit-law-add-ℤ :
    (k : ℤ) → Id (add-ℤ k zero-ℤ) k
  right-unit-law-add-ℤ (inl zero-ℕ) = refl
  right-unit-law-add-ℤ (inl (succ-ℕ x)) =
    ap pred-ℤ (right-unit-law-add-ℤ (inl x))
  right-unit-law-add-ℤ (inr (inl star)) = refl
  right-unit-law-add-ℤ (inr (inr zero-ℕ)) = refl
  right-unit-law-add-ℤ (inr (inr (succ-ℕ x))) =
    ap succ-ℤ (right-unit-law-add-ℤ (inr (inr x)))

{- Exercise 6.12 (b) asks to show the left and right predecessor and successor 
   laws. These are helpful to give proofs of associativity and commutativity. 
   -}

abstract
  left-predecessor-law-add-ℤ :
    (x y : ℤ) → Id (add-ℤ (pred-ℤ x) y) (pred-ℤ (add-ℤ x y))
  left-predecessor-law-add-ℤ (inl n) y = refl
  left-predecessor-law-add-ℤ (inr (inl star)) y = refl
  left-predecessor-law-add-ℤ (inr (inr zero-ℕ)) y =
    ( ap (λ t → add-ℤ t y) (left-inverse-pred-ℤ zero-ℤ)) ∙ 
    ( inv (left-inverse-pred-ℤ y))
  left-predecessor-law-add-ℤ (inr (inr (succ-ℕ x))) y =
    ( ap (λ t → (add-ℤ t y)) (left-inverse-pred-ℤ (inr (inr x)))) ∙
    ( inv (left-inverse-pred-ℤ (add-ℤ (inr (inr x)) y)))

  right-predecessor-law-add-ℤ :
    (x y : ℤ) → Id (add-ℤ x (pred-ℤ y)) (pred-ℤ (add-ℤ x y))
  right-predecessor-law-add-ℤ (inl zero-ℕ) n = refl
  right-predecessor-law-add-ℤ (inl (succ-ℕ m)) n =
    ap pred-ℤ (right-predecessor-law-add-ℤ (inl m) n)
  right-predecessor-law-add-ℤ (inr (inl star)) n = refl
  right-predecessor-law-add-ℤ (inr (inr zero-ℕ)) n =
    (right-inverse-pred-ℤ n) ∙ (inv (left-inverse-pred-ℤ n))
  right-predecessor-law-add-ℤ (inr (inr (succ-ℕ x))) n =
    ( ap succ-ℤ (right-predecessor-law-add-ℤ (inr (inr x)) n)) ∙
    ( ( right-inverse-pred-ℤ (add-ℤ (inr (inr x)) n)) ∙ 
      ( inv (left-inverse-pred-ℤ (add-ℤ (inr (inr x)) n))))

abstract
  left-successor-law-add-ℤ :
    (x y : ℤ) → Id (add-ℤ (succ-ℤ x) y) (succ-ℤ (add-ℤ x y))
  left-successor-law-add-ℤ (inl zero-ℕ) y =
    ( ap (λ t → add-ℤ t y) (right-inverse-pred-ℤ zero-ℤ)) ∙
    ( inv (right-inverse-pred-ℤ y))
  left-successor-law-add-ℤ (inl (succ-ℕ x)) y =
    ( inv (right-inverse-pred-ℤ (add-ℤ (inl x) y))) ∙
    ( ap succ-ℤ (inv (left-predecessor-law-add-ℤ (inl x) y)))
  left-successor-law-add-ℤ (inr (inl star)) y = refl
  left-successor-law-add-ℤ (inr (inr x)) y = refl

  right-successor-law-add-ℤ :
    (x y : ℤ) → Id (add-ℤ x (succ-ℤ y)) (succ-ℤ (add-ℤ x y))
  right-successor-law-add-ℤ (inl zero-ℕ) y =
    (left-inverse-pred-ℤ y) ∙ (inv (right-inverse-pred-ℤ y))
  right-successor-law-add-ℤ (inl (succ-ℕ x)) y =
    ( ap pred-ℤ (right-successor-law-add-ℤ (inl x) y)) ∙
    ( ( left-inverse-pred-ℤ (add-ℤ (inl x) y)) ∙
      ( inv (right-inverse-pred-ℤ (add-ℤ (inl x) y))))
  right-successor-law-add-ℤ (inr (inl star)) y = refl
  right-successor-law-add-ℤ (inr (inr zero-ℕ)) y = refl
  right-successor-law-add-ℤ (inr (inr (succ-ℕ x))) y =
    ap succ-ℤ (right-successor-law-add-ℤ (inr (inr x)) y)

{- Exercise 6.12 (c) asks to prove associativity and commutativity. Note that 
   we avoid an unwieldy amount of cases by only using induction on the first 
   argument. The resulting proof term is fairly short, and we don't have to 
   present ℤ as a certain quotient of ℕ × ℕ. -}

abstract
  associative-add-ℤ :
    (x y z : ℤ) → Id (add-ℤ (add-ℤ x y) z) (add-ℤ x (add-ℤ y z))
  associative-add-ℤ (inl zero-ℕ) y z =
    ( ap (λ t → add-ℤ t z) (left-predecessor-law-add-ℤ zero-ℤ y)) ∙
    ( ( left-predecessor-law-add-ℤ y z) ∙
      ( inv (left-predecessor-law-add-ℤ zero-ℤ (add-ℤ y z))))
  associative-add-ℤ (inl (succ-ℕ x)) y z =
    ( ap (λ t → add-ℤ t z) (left-predecessor-law-add-ℤ (inl x) y)) ∙
    ( ( left-predecessor-law-add-ℤ (add-ℤ (inl x) y) z) ∙
      ( ( ap pred-ℤ (associative-add-ℤ (inl x) y z)) ∙ 
        ( inv (left-predecessor-law-add-ℤ (inl x) (add-ℤ y z)))))
  associative-add-ℤ (inr (inl star)) y z = refl
  associative-add-ℤ (inr (inr zero-ℕ)) y z =
    ( ap (λ t → add-ℤ t z) (left-successor-law-add-ℤ zero-ℤ y)) ∙ 
    ( ( left-successor-law-add-ℤ y z) ∙ 
      ( inv (left-successor-law-add-ℤ zero-ℤ (add-ℤ y z))))
  associative-add-ℤ (inr (inr (succ-ℕ x))) y z =
    ( ap (λ t → add-ℤ t z) (left-successor-law-add-ℤ (inr (inr x)) y)) ∙
    ( ( left-successor-law-add-ℤ (add-ℤ (inr (inr x)) y) z) ∙
      ( ( ap succ-ℤ (associative-add-ℤ (inr (inr x)) y z)) ∙
        ( inv (left-successor-law-add-ℤ (inr (inr x)) (add-ℤ y z)))))

abstract
  commutative-add-ℤ :
    (x y : ℤ) → Id (add-ℤ x y) (add-ℤ y x)
  commutative-add-ℤ (inl zero-ℕ) y =
    ( left-predecessor-law-add-ℤ zero-ℤ y) ∙
    ( inv
      ( ( right-predecessor-law-add-ℤ y zero-ℤ) ∙
        ( ap pred-ℤ (right-unit-law-add-ℤ y))))
  commutative-add-ℤ (inl (succ-ℕ x)) y =
    ( ap pred-ℤ (commutative-add-ℤ (inl x) y)) ∙ 
    ( inv (right-predecessor-law-add-ℤ y (inl x)))
  commutative-add-ℤ (inr (inl star)) y = inv (right-unit-law-add-ℤ y)
  commutative-add-ℤ (inr (inr zero-ℕ)) y =
    inv
      ( ( right-successor-law-add-ℤ y zero-ℤ) ∙
        ( ap succ-ℤ (right-unit-law-add-ℤ y)))
  commutative-add-ℤ (inr (inr (succ-ℕ x))) y =
    ( ap succ-ℤ (commutative-add-ℤ (inr (inr x)) y)) ∙ 
    ( inv (right-successor-law-add-ℤ y (inr (inr x))))

{- Exercise 6.12 (d) finally asks to show the inverse laws, completing the 
   verification of the group laws. Combined with associativity and 
   commutativity we conclude that (add-ℤ x) and (λ x → add-ℤ x y) are 
   equivalences, for every x : ℤ and y : ℤ, respectively. -}

abstract
  left-inverse-law-add-ℤ :
    (x : ℤ) → Id (add-ℤ (neg-ℤ x) x) zero-ℤ
  left-inverse-law-add-ℤ (inl zero-ℕ) = refl
  left-inverse-law-add-ℤ (inl (succ-ℕ x)) =
    ( ap succ-ℤ (right-predecessor-law-add-ℤ (inr (inr x)) (inl x))) ∙ 
    ( ( right-inverse-pred-ℤ (add-ℤ (inr (inr x)) (inl x))) ∙
      ( left-inverse-law-add-ℤ (inl x))) 
  left-inverse-law-add-ℤ (inr (inl star)) = refl
  left-inverse-law-add-ℤ (inr (inr x)) =
    ( commutative-add-ℤ (inl x) (inr (inr x))) ∙ 
    ( left-inverse-law-add-ℤ (inl x))
  
  right-inverse-law-add-ℤ :
    (x : ℤ) → Id (add-ℤ x (neg-ℤ x)) zero-ℤ
  right-inverse-law-add-ℤ x =
    ( commutative-add-ℤ x (neg-ℤ x)) ∙ (left-inverse-law-add-ℤ x)

-- Similar for multiplication on ℤ

neg-neg-ℤ : (k : ℤ) → Id (neg-ℤ (neg-ℤ k)) k
neg-neg-ℤ (inl n) = refl
neg-neg-ℤ (inr (inl star)) = refl
neg-neg-ℤ (inr (inr n)) = refl

neg-pred-ℤ :
  (k : ℤ) → Id (neg-ℤ (pred-ℤ k)) (succ-ℤ (neg-ℤ k))
neg-pred-ℤ (inl x) = refl
neg-pred-ℤ (inr (inl star)) = refl
neg-pred-ℤ (inr (inr zero-ℕ)) = refl
neg-pred-ℤ (inr (inr (succ-ℕ x))) = refl

pred-neg-ℤ :
  (k : ℤ) → Id (pred-ℤ (neg-ℤ k)) (neg-ℤ (succ-ℤ k))
pred-neg-ℤ (inl zero-ℕ) = refl
pred-neg-ℤ (inl (succ-ℕ x)) = refl
pred-neg-ℤ (inr (inl star)) = refl
pred-neg-ℤ (inr (inr x)) = refl

right-negative-law-add-ℤ :
  (k l : ℤ) → Id (add-ℤ k (neg-ℤ l)) (neg-ℤ (add-ℤ (neg-ℤ k) l))
right-negative-law-add-ℤ (inl zero-ℕ) l =
  ( left-predecessor-law-add-ℤ zero-ℤ (neg-ℤ l)) ∙
  ( pred-neg-ℤ l)
right-negative-law-add-ℤ (inl (succ-ℕ x)) l =
  ( left-predecessor-law-add-ℤ (inl x) (neg-ℤ l)) ∙
  ( ( ap pred-ℤ (right-negative-law-add-ℤ (inl x) l)) ∙
    ( pred-neg-ℤ (add-ℤ (inr (inr x)) l)))
right-negative-law-add-ℤ (inr (inl star)) l = refl
right-negative-law-add-ℤ (inr (inr zero-ℕ)) l = inv (neg-pred-ℤ l)
right-negative-law-add-ℤ (inr (inr (succ-ℕ n))) l =
  ( left-successor-law-add-ℤ (in-pos n) (neg-ℤ l)) ∙
  ( ( ap succ-ℤ (right-negative-law-add-ℤ (inr (inr n)) l)) ∙
    ( inv (neg-pred-ℤ (add-ℤ (inl n) l))))

distributive-neg-add-ℤ :
  (k l : ℤ) → Id (neg-ℤ (add-ℤ k l)) (add-ℤ (neg-ℤ k) (neg-ℤ l))
distributive-neg-add-ℤ (inl zero-ℕ) l =
  ( ap neg-ℤ (left-predecessor-law-add-ℤ zero-ℤ l)) ∙
  ( neg-pred-ℤ l)
distributive-neg-add-ℤ (inl (succ-ℕ n)) l =
  ( neg-pred-ℤ (add-ℤ (inl n) l)) ∙
  ( ( ap succ-ℤ (distributive-neg-add-ℤ (inl n) l)) ∙
    ( ap (λ t → add-ℤ t (neg-ℤ l)) (inv (neg-pred-ℤ (inl n)))))
distributive-neg-add-ℤ (inr (inl star)) l = refl
distributive-neg-add-ℤ (inr (inr zero-ℕ)) l = inv (pred-neg-ℤ l)
distributive-neg-add-ℤ (inr (inr (succ-ℕ n))) l =
  ( inv (pred-neg-ℤ (add-ℤ (in-pos n) l))) ∙
  ( ap pred-ℤ (distributive-neg-add-ℤ (inr (inr n)) l))

left-zero-law-mul-ℤ : (k : ℤ) → Id (mul-ℤ zero-ℤ k) zero-ℤ
left-zero-law-mul-ℤ k = refl

right-zero-law-mul-ℤ : (k : ℤ) → Id (mul-ℤ k zero-ℤ) zero-ℤ
right-zero-law-mul-ℤ (inl zero-ℕ) = refl
right-zero-law-mul-ℤ (inl (succ-ℕ n)) =
  right-zero-law-mul-ℤ (inl n)
right-zero-law-mul-ℤ (inr (inl star)) = refl
right-zero-law-mul-ℤ (inr (inr zero-ℕ)) = refl
right-zero-law-mul-ℤ (inr (inr (succ-ℕ n))) =
  right-zero-law-mul-ℤ (inr (inr n))

left-unit-law-mul-ℤ : (k : ℤ) → Id (mul-ℤ one-ℤ k) k
left-unit-law-mul-ℤ k = refl

right-unit-law-mul-ℤ : (k : ℤ) → Id (mul-ℤ k one-ℤ) k
right-unit-law-mul-ℤ (inl zero-ℕ) = refl
right-unit-law-mul-ℤ (inl (succ-ℕ n)) =
  ap (add-ℤ (neg-one-ℤ)) (right-unit-law-mul-ℤ (inl n))
right-unit-law-mul-ℤ (inr (inl star)) = refl
right-unit-law-mul-ℤ (inr (inr zero-ℕ)) = refl
right-unit-law-mul-ℤ (inr (inr (succ-ℕ n))) =
  ap (add-ℤ one-ℤ) (right-unit-law-mul-ℤ (inr (inr n)))

left-neg-unit-law-mul-ℤ : (k : ℤ) → Id (mul-ℤ neg-one-ℤ k) (neg-ℤ k)
left-neg-unit-law-mul-ℤ k = refl

right-neg-unit-law-mul-ℤ : (k : ℤ) → Id (mul-ℤ k neg-one-ℤ) (neg-ℤ k)
right-neg-unit-law-mul-ℤ (inl zero-ℕ) = refl
right-neg-unit-law-mul-ℤ (inl (succ-ℕ n)) =
  ap (add-ℤ one-ℤ) (right-neg-unit-law-mul-ℤ (inl n))
right-neg-unit-law-mul-ℤ (inr (inl star)) = refl
right-neg-unit-law-mul-ℤ (inr (inr zero-ℕ)) = refl
right-neg-unit-law-mul-ℤ (inr (inr (succ-ℕ n))) =
  ap (add-ℤ neg-one-ℤ) (right-neg-unit-law-mul-ℤ (inr (inr n)))

left-successor-law-mul-ℤ :
  (k l : ℤ) → Id (mul-ℤ (succ-ℤ k) l) (add-ℤ l (mul-ℤ k l))
left-successor-law-mul-ℤ (inl zero-ℕ) l =
  inv (right-inverse-law-add-ℤ l)
left-successor-law-mul-ℤ (inl (succ-ℕ n)) l =
  ( ( inv (left-unit-law-add-ℤ (mul-ℤ (inl n) l))) ∙
    ( ap
      ( λ x → add-ℤ x (mul-ℤ (inl n) l))
      ( inv (right-inverse-law-add-ℤ l)))) ∙
  ( associative-add-ℤ l (neg-ℤ l) (mul-ℤ (inl n) l))
left-successor-law-mul-ℤ (inr (inl star)) l =
  inv (right-unit-law-add-ℤ l)
left-successor-law-mul-ℤ (inr (inr n)) l = refl

left-predecessor-law-mul-ℤ :
  (k l : ℤ) → Id (mul-ℤ (pred-ℤ k) l) (add-ℤ (neg-ℤ l) (mul-ℤ k l))
left-predecessor-law-mul-ℤ (inl n) l = refl
left-predecessor-law-mul-ℤ (inr (inl star)) l =
  ( left-neg-unit-law-mul-ℤ l) ∙
  ( inv (right-unit-law-add-ℤ (neg-ℤ l)))
left-predecessor-law-mul-ℤ (inr (inr zero-ℕ)) l =
  inv (left-inverse-law-add-ℤ l)
left-predecessor-law-mul-ℤ (inr (inr (succ-ℕ x))) l =
   ( ap
     ( λ t → add-ℤ t (mul-ℤ (in-pos x) l))
     ( inv (left-inverse-law-add-ℤ l))) ∙
   ( associative-add-ℤ (neg-ℤ l) l (mul-ℤ (in-pos x) l))

right-successor-law-mul-ℤ :
  (k l : ℤ) → Id (mul-ℤ k (succ-ℤ l)) (add-ℤ k (mul-ℤ k l))
right-successor-law-mul-ℤ (inl zero-ℕ) l = inv (pred-neg-ℤ l)
right-successor-law-mul-ℤ (inl (succ-ℕ n)) l =
  ( left-predecessor-law-mul-ℤ (inl n) (succ-ℤ l)) ∙
  ( ( ap (add-ℤ (neg-ℤ (succ-ℤ l))) (right-successor-law-mul-ℤ (inl n) l)) ∙
    ( ( inv (associative-add-ℤ (neg-ℤ (succ-ℤ l)) (inl n) (mul-ℤ (inl n) l))) ∙
      ( ( ap
          ( λ t → add-ℤ t (mul-ℤ (inl n) l))
          { x = add-ℤ (neg-ℤ (succ-ℤ l)) (inl n)}
          { y = add-ℤ (inl (succ-ℕ n)) (neg-ℤ l)}
          ( ( right-successor-law-add-ℤ (neg-ℤ (succ-ℤ l)) (inl (succ-ℕ n))) ∙
            ( ( ap succ-ℤ
                ( commutative-add-ℤ (neg-ℤ (succ-ℤ l)) (inl (succ-ℕ n)))) ∙
              ( ( inv
                  ( right-successor-law-add-ℤ
                    ( inl (succ-ℕ n))
                    ( neg-ℤ (succ-ℤ l)))) ∙
                ( ap
                  ( add-ℤ (inl (succ-ℕ n)))
                  ( ( ap succ-ℤ (inv (pred-neg-ℤ l))) ∙
                    ( right-inverse-pred-ℤ (neg-ℤ l)))))))) ∙
        ( associative-add-ℤ (inl (succ-ℕ n)) (neg-ℤ l) (mul-ℤ (inl n) l)))))
right-successor-law-mul-ℤ (inr (inl star)) l = refl
right-successor-law-mul-ℤ (inr (inr zero-ℕ)) l = refl
right-successor-law-mul-ℤ (inr (inr (succ-ℕ n))) l =
  ( left-successor-law-mul-ℤ (in-pos n) (succ-ℤ l)) ∙
  ( ( ap (add-ℤ (succ-ℤ l)) (right-successor-law-mul-ℤ (inr (inr n)) l)) ∙
    ( ( inv (associative-add-ℤ (succ-ℤ l) (in-pos n) (mul-ℤ (in-pos n) l))) ∙
      ( ( ap
          ( λ t → add-ℤ t (mul-ℤ (in-pos n) l))
          { x = add-ℤ (succ-ℤ l) (in-pos n)}
          { y = add-ℤ (in-pos (succ-ℕ n)) l}
          ( ( left-successor-law-add-ℤ l (in-pos n)) ∙
            ( ( ap succ-ℤ (commutative-add-ℤ l (in-pos n))) ∙
              ( inv (left-successor-law-add-ℤ (in-pos n) l))))) ∙
        ( associative-add-ℤ (inr (inr (succ-ℕ n))) l (mul-ℤ (inr (inr n)) l)))))

right-predecessor-law-mul-ℤ :
  (k l : ℤ) → Id (mul-ℤ k (pred-ℤ l)) (add-ℤ (neg-ℤ k) (mul-ℤ k l))
right-predecessor-law-mul-ℤ (inl zero-ℕ) l =
  ( left-neg-unit-law-mul-ℤ (pred-ℤ l)) ∙
  ( neg-pred-ℤ l)
right-predecessor-law-mul-ℤ (inl (succ-ℕ n)) l =
  ( left-predecessor-law-mul-ℤ (inl n) (pred-ℤ l)) ∙
  ( ( ap (add-ℤ (neg-ℤ (pred-ℤ l))) (right-predecessor-law-mul-ℤ (inl n) l)) ∙
    ( ( inv
        ( associative-add-ℤ (neg-ℤ (pred-ℤ l)) (in-pos n) (mul-ℤ (inl n) l))) ∙
      ( ( ap
          ( λ t → add-ℤ t (mul-ℤ (inl n) l))
          { x = add-ℤ (neg-ℤ (pred-ℤ l)) (inr (inr n))}
          { y = add-ℤ (neg-ℤ (inl (succ-ℕ n))) (neg-ℤ l)}
          ( ( ap (λ t → add-ℤ t (in-pos n)) (neg-pred-ℤ l)) ∙
            ( ( left-successor-law-add-ℤ (neg-ℤ l) (in-pos n)) ∙
              ( ( ap succ-ℤ (commutative-add-ℤ (neg-ℤ l) (in-pos n))) ∙
                ( inv (left-successor-law-add-ℤ (in-pos n) (neg-ℤ l))))))) ∙
        ( associative-add-ℤ (in-pos (succ-ℕ n)) (neg-ℤ l) (mul-ℤ (inl n) l)))))
right-predecessor-law-mul-ℤ (inr (inl star)) l = refl
right-predecessor-law-mul-ℤ (inr (inr zero-ℕ)) l = refl
right-predecessor-law-mul-ℤ (inr (inr (succ-ℕ n))) l =
  ( left-successor-law-mul-ℤ (in-pos n) (pred-ℤ l)) ∙
  ( ( ap (add-ℤ (pred-ℤ l)) (right-predecessor-law-mul-ℤ (inr (inr n)) l)) ∙
    ( ( inv (associative-add-ℤ (pred-ℤ l) (inl n) (mul-ℤ (inr (inr n)) l))) ∙
      ( ( ap
          ( λ t → add-ℤ t (mul-ℤ (in-pos n) l))
          { x = add-ℤ (pred-ℤ l) (inl n)}
          { y = add-ℤ (neg-ℤ (in-pos (succ-ℕ n))) l}
          ( ( left-predecessor-law-add-ℤ l (inl n)) ∙
            ( ( ap pred-ℤ (commutative-add-ℤ l (inl n))) ∙
              ( inv (left-predecessor-law-add-ℤ (inl n) l))))) ∙
        ( associative-add-ℤ (inl (succ-ℕ n)) l (mul-ℤ (inr (inr n)) l)))))

right-distributive-mul-add-ℤ :
  (k l m : ℤ) → Id (mul-ℤ (add-ℤ k l) m) (add-ℤ (mul-ℤ k m) (mul-ℤ l m))
right-distributive-mul-add-ℤ (inl zero-ℕ) l m =
  ( left-predecessor-law-mul-ℤ l m) ∙
  ( ap
    ( λ t → add-ℤ t (mul-ℤ l m))
    ( inv
      ( ( left-predecessor-law-mul-ℤ zero-ℤ m) ∙
        ( right-unit-law-add-ℤ (neg-ℤ m)))))
right-distributive-mul-add-ℤ (inl (succ-ℕ x)) l m =
  ( left-predecessor-law-mul-ℤ (add-ℤ (inl x) l) m) ∙
  ( ( ap (add-ℤ (neg-ℤ m)) (right-distributive-mul-add-ℤ (inl x) l m)) ∙
    ( inv (associative-add-ℤ (neg-ℤ m) (mul-ℤ (inl x) m) (mul-ℤ l m))))
right-distributive-mul-add-ℤ (inr (inl star)) l m = refl
right-distributive-mul-add-ℤ (inr (inr zero-ℕ)) l m =
  left-successor-law-mul-ℤ l m
right-distributive-mul-add-ℤ (inr (inr (succ-ℕ n))) l m =
  ( left-successor-law-mul-ℤ (add-ℤ (in-pos n) l) m) ∙
  ( ( ap (add-ℤ m) (right-distributive-mul-add-ℤ (inr (inr n)) l m)) ∙
    ( inv (associative-add-ℤ m (mul-ℤ (in-pos n) m) (mul-ℤ l m))))

left-negative-law-mul-ℤ :
  (k l : ℤ) → Id (mul-ℤ (neg-ℤ k) l) (neg-ℤ (mul-ℤ k l))
left-negative-law-mul-ℤ (inl zero-ℕ) l =
  ( left-unit-law-mul-ℤ l) ∙
  ( inv (neg-neg-ℤ l))
left-negative-law-mul-ℤ (inl (succ-ℕ n)) l =
  ( ap (λ t → mul-ℤ t l) (neg-pred-ℤ (inl n))) ∙
  ( ( left-successor-law-mul-ℤ (neg-ℤ (inl n)) l) ∙
    ( ( ap (add-ℤ l) (left-negative-law-mul-ℤ (inl n) l)) ∙
      ( right-negative-law-add-ℤ l (mul-ℤ (inl n) l))))
left-negative-law-mul-ℤ (inr (inl star)) l = refl
left-negative-law-mul-ℤ (inr (inr zero-ℕ)) l = refl
left-negative-law-mul-ℤ (inr (inr (succ-ℕ n))) l =
  ( left-predecessor-law-mul-ℤ (inl n) l) ∙
  ( ( ap (add-ℤ (neg-ℤ l)) (left-negative-law-mul-ℤ (inr (inr n)) l)) ∙
    ( inv (distributive-neg-add-ℤ l (mul-ℤ (in-pos n) l))))

associative-mul-ℤ :
  (k l m : ℤ) → Id (mul-ℤ (mul-ℤ k l) m) (mul-ℤ k (mul-ℤ l m))
associative-mul-ℤ (inl zero-ℕ) l m =
  left-negative-law-mul-ℤ l m
associative-mul-ℤ (inl (succ-ℕ n)) l m =
  ( right-distributive-mul-add-ℤ (neg-ℤ l) (mul-ℤ (inl n) l) m) ∙
  ( ( ap (add-ℤ (mul-ℤ (neg-ℤ l) m)) (associative-mul-ℤ (inl n) l m)) ∙
    ( ap
      ( λ t → add-ℤ t (mul-ℤ (inl n) (mul-ℤ l m)))
      ( left-negative-law-mul-ℤ l m)))
associative-mul-ℤ (inr (inl star)) l m = refl
associative-mul-ℤ (inr (inr zero-ℕ)) l m = refl
associative-mul-ℤ (inr (inr (succ-ℕ n))) l m =
  ( right-distributive-mul-add-ℤ l (mul-ℤ (in-pos n) l) m) ∙
  ( ap (add-ℤ (mul-ℤ l m)) (associative-mul-ℤ (inr (inr n)) l m))

commutative-mul-ℤ :
  (k l : ℤ) → Id (mul-ℤ k l) (mul-ℤ l k)
commutative-mul-ℤ (inl zero-ℕ) l = inv (right-neg-unit-law-mul-ℤ l)
commutative-mul-ℤ (inl (succ-ℕ n)) l =
  ( ap (add-ℤ (neg-ℤ l)) (commutative-mul-ℤ (inl n) l)) ∙
  ( inv (right-predecessor-law-mul-ℤ l (inl n)))
commutative-mul-ℤ (inr (inl star)) l = inv (right-zero-law-mul-ℤ l)
commutative-mul-ℤ (inr (inr zero-ℕ)) l = inv (right-unit-law-mul-ℤ l)
commutative-mul-ℤ (inr (inr (succ-ℕ n))) l =
  ( ap (add-ℤ l) (commutative-mul-ℤ (inr (inr n)) l)) ∙
  ( inv (right-successor-law-mul-ℤ l (in-pos n)))
